Remove existence of the [gpointer] and [gpointer_or_null] types

ind/Gpointers.fst
@@ -1,46 +1,44 @@
 module Gpointers
 
+open LowStar.Buffer
 module HS = FStar.HyperStack
 module ST = FStar.HyperStack.ST
 module B = LowStar.Buffer
 module BO = LowStar.BufferOps
 module Mod = LowStar.Modifies
 
-type gpointer t = B.pointer t
-type gpointer_or_null t = B.pointer_or_null t
+let disjoint (#t:Type) (a b: pointer t) = B.as_addr a <> B.as_addr b
 
-let disjoint (#t:Type) (a b: gpointer t) = B.as_addr a <> B.as_addr b
+let null #t : pointer_or_null t = B.null #t
 
-let null #t : gpointer_or_null t = B.null #t
+assume val is_null (p:pointer_or_null 't) : Tot (b:bool{b <==> p == null})
+let is_not_null (p:pointer_or_null 't) = not (is_null p)
 
-assume val is_null (p:gpointer_or_null 't) : Tot (b:bool{b <==> p == null})
-let is_not_null (p:gpointer_or_null 't) = not (is_null p)
-
-let lemma_is_null (p:gpointer_or_null 't) :
+let lemma_is_null (p:pointer_or_null 't) :
   Lemma
     (ensures (is_null p <==> B.g_is_null p))
     [SMTPat (is_null p)]
     = B.null_unique p
 
 let test_null #t =
-  let p : gpointer_or_null t = null in
+  let p : pointer_or_null t = null in
   assert (is_null p)
 
 val non_null:
   #t:Type ->
-  a:gpointer_or_null t{is_not_null a} ->
-  b:gpointer t
+  a:pointer_or_null t{is_not_null a} ->
+  b:pointer t
 let non_null #t a = a
 
 val lemma_non_null :
   #t:Type ->
-  a:gpointer_or_null t{is_not_null a} ->
+  a:pointer_or_null t{is_not_null a} ->
   Lemma (ensures (a == non_null a))
     [SMTPat (non_null a)]
 let lemma_non_null #t a = ()
 
 val of_non_null:
   #t:Type ->
-  a:gpointer t ->
-  b:gpointer_or_null t
+  a:pointer t ->
+  b:pointer_or_null t
 let of_non_null #t a = a
